Relaxation Boilerplate Relaxation Formula functionality Temporarily reduced dependencies with normalization definitions

Formula_Utils.thy
@@ -11,6 +11,86 @@ fun is_conj where
   "is_conj (F \<^bold>\<and> G) \<longleftrightarrow> is_lit_plus F \<and> is_conj G" |
   "is_conj H \<longleftrightarrow> is_lit_plus H"
 
+
+(* assumes the argument to be in a right-deep tree, i.e. is_conj *)
+(* possible optimization: un_and (Not Bot) = []" *)
+(* still is defined and preserves semantics if argument isn't a pure right conjunction *)
+fun un_and :: "'a formula \<Rightarrow> 'a formula list" where
+  "un_and (F \<^bold>\<and> G) = F # un_and G" |
+  "un_and F = [F]"
+
+lemma "is_conj F \<Longrightarrow> \<forall>f \<in> set (un_and F). is_lit_plus f"
+  by (induction F rule: is_conj.induct) simp_all
+
+lemma un_and_sem: "A \<Turnstile> F \<longleftrightarrow> (\<forall>f \<in> set (un_and F). A \<Turnstile> f)"
+  by (induction F) simp_all
+
+fun is_lit_pos :: "'a formula \<Rightarrow> bool" where
+  "is_lit_pos \<bottom> = True" |
+  "is_lit_pos (Not \<bottom>) = True" |
+  "is_lit_pos (Atom _) = True" |
+  "is_lit_pos _ = False"
+
+lemma lit_pos_vs_plus: "is_lit_pos l = is_lit_plus l \<or> (\<exists>a. l = \<^bold>\<not> (Atom a))"
+  by (cases l rule: is_lit_plus.cases) simp_all
+
+fun is_pos_conj :: "'a formula \<Rightarrow> bool" where
+  "is_pos_conj (F \<^bold>\<and> G) \<longleftrightarrow> is_lit_pos F \<and> is_pos_conj G" |
+  "is_pos_conj F \<longleftrightarrow> is_lit_pos F"
+
+lemma pos_conj_conj: "is_pos_conj F \<Longrightarrow> is_conj F"
+  apply (induction F rule: is_conj.induct) using lit_pos_vs_plus apply force
+  apply simp_all using lit_pos_vs_plus by force
+
+lemma "is_pos_conj F \<Longrightarrow> \<forall>f \<in> set (un_and F). is_lit_pos f"
+  by (induction F rule: is_conj.induct) simp_all
+
+(* This is only defined for pure conjunctive clauses. *)
+(* TODO maybe extend the definition for other use cases? *)
+
+fun relax_lit :: "'a formula \<Rightarrow> 'a formula" where
+  "relax_lit \<bottom> = \<^bold>\<not> \<bottom>" |
+  "relax_lit (\<^bold>\<not> \<bottom>) = \<^bold>\<not> \<bottom>" |
+  "relax_lit (Atom a) = Atom a" |
+  "relax_lit (\<^bold>\<not> (Atom a)) = \<^bold>\<not> \<bottom>"
+
+lemma relax_lit_pos: "is_lit_plus f \<Longrightarrow> is_lit_pos (relax_lit f)"
+  by (cases f rule: relax_lit.cases) simp_all
+
+(* also only defined for is_conj *)
+fun relax_conj :: "'a formula \<Rightarrow> 'a formula" where
+  "relax_conj (F \<^bold>\<and> G) = relax_lit F \<^bold>\<and> relax_conj G" |
+  "relax_conj f = relax_lit f"
+
+lemma relax_conj_pos: "is_conj F \<Longrightarrow> is_pos_conj (relax_conj F)"
+  apply (induction F rule: is_conj.induct) apply (simp_all add: relax_lit_pos)
+  subgoal for v apply (cases v) apply simp_all done done
+
+(* can probably think of a stronger property *)
+lemma relax_conj_un_conj:
+  assumes "is_conj F"
+  shows "set (un_and (relax_conj F)) \<subseteq> \<^bold>\<not>\<bottom> \<triangleright> set (un_and F)"
+  using assms proof (induction F rule: is_conj.induct)
+  case (1 F G) thus ?case
+    apply (cases F) apply auto[6] subgoal for x by (cases x) simp_all
+    done
+next
+  case ("2_3" v)
+  then show ?case by (cases v) simp_all
+qed simp_all
+
+lemma relax_conj_sem:
+  assumes "is_conj F"
+  shows "A \<Turnstile> F \<Longrightarrow> A \<Turnstile> relax_conj F"
+proof -
+  have "A \<Turnstile> relax_conj F \<longleftrightarrow> (\<forall>l \<in> set (un_and (relax_conj F)). A \<Turnstile> l)"
+    using un_and_sem by blast
+  hence "(\<forall>l \<in> \<^bold>\<not>\<bottom> \<triangleright> set (un_and F). A \<Turnstile> l) \<Longrightarrow> A \<Turnstile> relax_conj F"
+    using assms using relax_conj_un_conj by blast
+  thus "A \<Turnstile> F \<Longrightarrow> A \<Turnstile> relax_conj F" using un_and_sem by auto
+qed
+
+
 lemma map_preserves_isconj:
   assumes "is_conj F" shows "is_conj (map_formula m F)"
 using assms proof (induction F)
